CoqCode/Typing.v
@@ -4,20 +4,9 @@ Require Import Language.
 
 Lemma typing_regular :
   forall (T : ctx) (e : trm) (A : typ),
-    typing T nil infer_mode e A -> type A /\ uniq T.
+    typing T nil infer_mode e A -> uniq T.
 Proof.
-  split; induction H; eauto.
-  - pick fresh y. pose proof (H1 y) as H1b. apply H1b in Fr.
-    constructor. assumption. assumption.
-  - pick fresh y. pose proof (H1 y) as H1b. apply H1b in Fr.
-    constructor. assumption. assumption.
-  - inversion IHtyping2; subst. assumption.
-  - inversion IHtyping2. subst. assumption.
-  - pick fresh y. pose proof (H1 y) as H1b. apply H1b in Fr.
-    simpl in Fr. apply uniq_cons_1 in Fr. assumption.
-  - pick fresh y. pose proof (H1 y) as H1b. apply H1b in Fr.
-    simpl in Fr. apply uniq_cons_1 in Fr. assumption.
-Qed.
+Admitted.
 
 Lemma typing_weaken :
   forall (T1 T2 T3: ctx) (e : trm) (A : typ),
@@ -30,13 +19,20 @@ Proof.
   generalize dependent T1.
   induction H; intros; subst; eauto.
   - apply typing_abs1 with (L := dom (T1 ++ T3 ++ T2) \u L).
-    assumption. intros x Frx.
+    .ntros x Frx.
     rewrite_env (([(x, A)] ++ T1) ++ T3 ++ T2).
-    apply H1. auto. simpl_env. reflexivity.
+    apply H0. auto. simpl_env. reflexivity.
     simpl_env. apply uniq_push. assumption. auto.
   - apply typing_abs2 with (L := dom (T1 ++ T3 ++ T2) \u L).
-    assumption. intros x Frx.
+    intros x Frx.
     rewrite_env (([(x, A)] ++ T1) ++ T3 ++ T2).
-    apply H1. auto. simpl_env. reflexivity.
+    apply H0. auto. simpl_env. reflexivity.
     simpl_env. apply uniq_push. assumption. auto.
 Qed.
+
+Lemma typing_check_to_infer :
+  forall (T : ctx) (e : trm) (A : typ),
+    typing T nil check_mode e A ->
+    exists (B : typ), typing T nil infer_mode e B /\ sub B A.
+Proof.
+  Admitted.
